tests/lean/run/mangling.lean
@@ -1,5 +1,7 @@
 module
-import Lean.Compiler.NameMangling
+import all Lean.Compiler.NameMangling
+import all Init.Data.String.Basic
+import all Init.Data.Repr
 
 /-!
 # Test behavior of name mangling
@@ -87,3 +89,219 @@ Anonymous vs empty string
 #eval checkMangle .anonymous ""
 #eval checkMangle `«» "00"
 #eval checkMangle `«».«» "00_00"
+
+@[simp]
+theorem String.append_right_inj {t₁ t₂ : String} (s : String) : s ++ t₁ = s ++ t₂ ↔ t₁ = t₂ := by
+  simp [ByteArray.append_right_inj, ← String.bytes_inj]
+
+def String.posBetween (s t : String) : (s ++ t).ValidPos :=
+  ⟨s.endPos, by simp [Pos.Raw.isValid_append]⟩
+
+@[simp]
+theorem String.posBetween_eq_endValidPos_iff (s t : String) :
+    s.posBetween t = (s ++ t).endValidPos ↔ t = "" := by
+  simp [String.ValidPos.ext_iff, String.Pos.Raw.ext_iff, String.posBetween]
+
+@[simp]
+theorem String.length_eq_zero_iff {s : String} : s.length = 0 ↔ s = "" := by
+  simp [← String.length_data]
+
+@[simp]
+theorem String.append_eq_empty_iff {s t : String} : s ++ t = "" ↔ s = "" ∧ t = "" := by
+  simp [← String.bytes_inj]
+
+@[simp]
+theorem String.get_posBetween_singleton_append {s t : String} {c : Char} (h) :
+    (s.posBetween (String.singleton c ++ t)).get h = c := by
+  simp only [ValidPos.get, Slice.Pos.get, str_toSlice, startInclusive_toSlice, offset_startValidPos,
+    Pos.Raw.byteIdx_zero, posBetween, ValidPos.offset_toSlice, byteIdx_endPos, Nat.zero_add]
+  simp only [decodeChar, bytes_append, bytes_singleton, ByteArray.utf8DecodeChar]
+  rw [← Option.some.injEq, Option.some_get, ByteArray.utf8DecodeChar?_eq_utf8DecodeChar?_extract]
+  rw [← String.size_bytes, ByteArray.extract_append_eq_right rfl (by simp)]
+  rw [List.utf8DecodeChar?_utf8Encode_singleton_append]
+
+@[simp]
+theorem String.next_posBetween_singleton_append {s t : String} {c : Char} (h) :
+    (s.posBetween (String.singleton c ++ t)).next h =
+      ((s.push c).posBetween t).cast (by simp only [String.push_eq_append, String.append_assoc]) := by
+  simp only [ValidPos.next, ValidPos.ext_iff, Slice.Pos.ofset_ofSlice, ValidPos.offset_cast,
+    Pos.Raw.ext_iff, Slice.Pos.byteIdx_offset_next, ValidPos.offset_toSlice]
+  rw [← String.ValidPos.get.eq_def _ h, String.get_posBetween_singleton_append]
+  simp [String.posBetween]
+
+def encodeHex (n val : Nat) : String :=
+  match n with
+  | 0 => ""
+  | k + 1 => (String.singleton <| Nat.digitChar (val / 16 ^ k)) ++ encodeHex k (val % 16 ^ k)
+
+@[simp]
+theorem String.push_ne_empty : String.push s c ≠ "" := by
+  simp [← String.bytes_inj]
+
+@[simp]
+theorem String.singleton_ne_empty : String.singleton c ≠ "" := by
+  simp [← String.bytes_inj]
+
+@[simp]
+theorem checkLowerHex_uncast {s t : String} {p : t.ValidPos} (h : t = s) :
+    Lean.checkLowerHex n s (p.cast h) = Lean.checkLowerHex n t p := by
+  cases h; rfl
+
+@[simp]
+theorem parseLowerHex_uncast {s t : String} {p : t.ValidPos} (h : t = s) (h') :
+    Lean.parseLowerHex n s (p.cast h) h' i = Lean.parseLowerHex n t p (by cases h; exact h') i := by
+  cases h; rfl
+
+theorem checkLowerHex_encodeHex (h : val < 16 ^ n) :
+    Lean.checkLowerHex n (s ++ encodeHex n val) (String.posBetween _ _) = true := by
+  fun_induction encodeHex generalizing s
+  · rfl
+  · rename_i val k ih
+    have h' : val % 16 ^ k < 16 ^ k := Nat.mod_lt _ (Nat.pow_pos (by decide))
+    suffices (val / 16 ^ k).digitChar.isDigit = true ∨
+        97 ≤ (val / 16 ^ k).digitChar.val ∧ (val / 16 ^ k).digitChar.val ≤ 102 by
+      simpa [Lean.checkLowerHex, ih h']
+    rw [Nat.pow_succ] at h
+    have h'' : val / 16 ^ k < 16 := by
+      rwa [Nat.div_lt_iff_lt_mul (Nat.pow_pos (by decide)), Nat.mul_comm]
+    generalize val / 16 ^ k = c at h''
+    decide +revert
+
+theorem Nat.digitChar_eq (n : Nat) (h : n < 16) : n.digitChar =
+    if h : n < 10 then
+      ⟨UInt32.ofNatLT (48 + n) (by grind), by grind [UInt32.toNat_ofNatLT]⟩
+    else
+      ⟨UInt32.ofNatLT (87 + n) (by grind), by grind [UInt32.toNat_ofNatLT]⟩ := by
+  decide +revert
+
+theorem Nat.shiftLeft_or_eq_add (a b c : Nat) (h : c < 2 ^ b) :
+    (a <<< b) ||| c = a * 2 ^ b + c := by
+  refine Nat.eq_of_testBit_eq fun i => ?_
+  rw (occs := [2]) [Nat.testBit_eq_decide_div_mod_eq]
+  rw [Bool.eq_iff_iff, decide_eq_true_eq]
+  simp only [testBit_or, testBit_shiftLeft, ge_iff_le, Bool.or_eq_true, Bool.and_eq_true,
+    decide_eq_true_eq]
+  by_cases hb : b ≤ i
+  · have : c.testBit i = false := by
+      rw [Nat.testBit_eq_decide_div_mod_eq, decide_eq_false_iff_not, Nat.div_eq_of_lt]
+      · decide
+      · exact Nat.lt_of_lt_of_le h (Nat.pow_le_pow_right (by decide) hb)
+    simp only [hb, true_and, this, Bool.false_eq_true, or_false]
+    obtain ⟨i, rfl⟩ := hb.dest
+    simp [Nat.pow_add, ← Nat.div_div_eq_div_mul, Nat.add_comm _ c, Nat.add_mul_div_right,
+      Nat.two_pow_pos, Nat.div_eq_of_lt h, Nat.testBit_eq_decide_div_mod_eq]
+  · simp only [hb, false_and, false_or]
+    simp only [Nat.not_le] at hb
+    obtain ⟨d, rfl⟩ := hb.dest
+    rw [Nat.succ_add, ← Nat.add_succ, Nat.pow_add', ← Nat.mul_assoc, Nat.add_comm,
+      Nat.add_mul_div_right _ _ (Nat.two_pow_pos _), ← Nat.add_mod_mod, Nat.pow_succ,
+      ← Nat.mul_assoc, Nat.mul_mod_left, Nat.add_zero, testBit_eq_decide_div_mod_eq,
+      decide_eq_true_eq]
+
+theorem parseLowerHex_encodeHex (h : val < 16 ^ n) (h') :
+    Lean.parseLowerHex n (s ++ encodeHex n val) (String.posBetween _ _) h' i =
+        i * 16 ^ n + val := by
+  fun_induction encodeHex generalizing s i
+  · simp_all [Lean.parseLowerHex]
+  · rename_i val k ih
+    have h' : val % 16 ^ k < 16 ^ k := Nat.mod_lt _ (Nat.pow_pos (by decide))
+    simp [Lean.parseLowerHex, ih h']
+    rw [Nat.pow_succ] at h
+    have h'' : val / 16 ^ k < 16 := by
+      rwa [Nat.div_lt_iff_lt_mul (Nat.pow_pos (by decide)), Nat.mul_comm]
+    rw [Nat.mod_eq_sub]
+    generalize hc : val / 16 ^ k = c at h''
+    rw [Char.isDigit]
+    simp only [ge_iff_le, Bool.and_eq_true, decide_eq_true_eq]
+    have this (a h) := Nat.shiftLeft_or_eq_add i 4 a h
+    simp only [Nat.reducePow] at this
+    rw [Nat.pow_succ, Nat.mul_comm _ 16, ← Nat.mul_assoc, ← apply_ite (· + _)]
+    have : i * 16 * 16 ^ k + val = (i * 16 + c) * 16 ^ k + (val - 16 ^ k * c) := by
+      rw [Nat.add_mul, Nat.mul_comm c, Nat.add_assoc, Nat.add_sub_cancel']
+      rw [← hc, Nat.mul_comm]
+      exact Nat.div_mul_le_self val (16 ^ k)
+    rw [this, Nat.add_right_cancel_iff]; clear this
+    rw [← this c h'']; clear this hc
+    split <;> (congr; decide +revert)
+
+def Char.mangle (c : Char) : String :=
+  if c.isDigit ∨ c.isAlpha then String.singleton c
+  else if c = '_' then "__"
+  else if c.val < 0x100 then "_x" ++ encodeHex 2 c.toNat
+  else if c.val < 0x10000 then "_u" ++ encodeHex 4 c.toNat
+  else "_U" ++ encodeHex 8 c.toNat
+
+theorem String.something_uhh (n : Nat) (h : n < 16 ^ k) :
+    List.foldl (fun r c => r.push c)
+      (Nat.repeat (fun x => x.push '0') (k - (Nat.toDigits 16 n).length) (s ++ "_U"))
+      (Nat.toDigits 16 n) = encodeHex k n := by
+  sorry
+
+#check (rfl : Lean.Name.mangle `abc.c == "abc_c")
+
+theorem String.mangleAux_normalize : mangleAux n it s = s ++ mangleAux n it "" := by
+  induction n generalizing it s with
+  | zero => simp [String.mangleAux]
+  | succ k ih =>
+    unfold String.mangleAux
+    extract_lets
+    split
+    · conv => lhs; rw [ih]
+      conv => rhs; rw [ih]
+      simp only [String.push_eq_append, String.empty_append, String.append_assoc]
+    split
+    · conv => lhs; rw [ih]
+      conv => rhs; rw [ih]
+      simp only [String.empty_append, String.append_assoc]
+    split
+    · conv => lhs; rw [ih]
+      conv => rhs; rw [ih]
+      simp +zetaDelta only [String.push_eq_append, String.empty_append, String.append_assoc]
+    split
+    · conv => lhs; rw [ih]
+      conv => rhs; rw [ih]
+      simp +zetaDelta only [String.push_eq_append, String.empty_append, String.append_assoc]
+    · conv => lhs; rw [ih]
+      conv => rhs; rw [ih]
+      simp +zetaDelta only [String.push_eq_append, String.empty_append, String.append_assoc]
+
+theorem String.mangle_eq_empty : mangle s = "" ↔ s = "" := by
+  rw [String.mangle]
+  generalize hlen : s.length = len
+  generalize hit : s.mkIterator = it
+  generalize hacc : "" = acc
+  fun_cases String.mangleAux <;> subst hacc hit
+  · simp_all
+  ·
+
+#print String.mangleAux.fun_cases_unfolding
+
+namespace Lean.Name
+
+theorem mangleAux_eq_empty : mangleAux nm = "" ↔ nm = .anonymous := by
+  constructor
+  rotate_left
+  · rintro rfl; rfl
+  fun_cases mangleAux
+  · simp
+  · simp
+  · rename_i s m h
+
+mutual
+
+theorem nameStart_thm (hn : (mangleAux nm).length ≤ n) :
+    unmangleAux.nameStart (s ++ mangleAux nm) (s.endValidPos.appendRight _) res n = res ++ nm := by
+  fun_cases unmangleAux.nameStart
+  · simp at hn
+
+end
+
+theorem unmangle_mangleAux (n : Name) : unmangle n.mangleAux = n := by
+  sorry
+
+theorem mangle_inj {n n' : Name} : n.mangle = n'.mangle ↔ n = n' := by
+  simp only [mangle, String.append_right_inj]
+  constructor
+  · intro h
+    simpa [unmangle_mangleAux] using congrArg unmangle h
+  · exact congrArg mangleAux
